#+TITLE: Econ202A Assignment 1
#+AUTHOR: Chris Ackerman
#+LATEX_HEADER: \usepackage{amsthm}
#+LATEX_HEADER: \usepackage{url}
#+LATEX_HEADER: \newtheorem*{definition}{Definition}
#+LATEX_HEADER: \newtheorem*{example}{Example}
#+LATEX_HEADER: \newtheorem*{theorem}{Theorem}
#+LATEX_HEADER: \newtheorem*{exercise}{Exercise}
#+LATEX_HEADER: \newtheorem{question}{Question}
#+LATEX_HEADER: \usepackage[margin=1.25in]{geometry}
#+LATEX_HEADER: \usepackage{hyperref} % Required for adding links	and customizing them
#+LATEX_HEADER: \usepackage[dvipsnames]{xcolor}
#+LATEX_HEADER: \usepackage{booktabs}
#+LATEX_HEADER: \usepackage{enumitem}
#+LATEX_HEADER: \newcommand{\gr}{\textcolor{ForestGreen}}
#+LATEX_HEADER: \newcommand{\rd}{\textcolor{red}}
#+LATEX_HEADER: \newcommand{\R}{\mathbb{R}}
#+LATEX_HEADER: \newcommand{\frall}{\ \forall}
#+OPTIONS:  ':t

  \newpage
* Problem 1
  #+BEGIN_SRC latex
  Consider the following problem solved be a representative agent:
  \begin{align*}
  \max \sum^\infty_{t = 0} &\beta^t \log c_t, \quad 0 < \beta < 1\\
\intertext{subject to}
c_t + k_{t + 1} &\le k^\theta_t, \quad 0 < \theta < 1,\\
k_0 &\text{ given.}
  \end{align*}
  \begin{enumerate}[label=(\alph*)]
    \item $ $
    \begin{align}
%     v(k_0) &= \max(u(c_0) + \beta v(k_1))\\
% v(k_0) &= \max(u(f(k_0) - k_1) + \beta v(k_1))\\
% u'(f(k_0) - k_1) &= \beta v'(k_1)\\
% F(k_t) &= k_t^\theta\\
U'(f(k_t) - k_{t + 1}) &= \beta U' (f(k_{t + 1}) - k_{t + 2})f'(k_{t + 1}) \tag{Euler Equation}\\
\frac{1}{k^\theta_t - k_{t + 1}} &= \beta \frac{\theta k^{\theta - 1}_{t + 1}}{k^\theta_{t + 1} - k_{t + 2}}\\
\frac{1}{k^\theta_{T - 1} - k_T} &= \beta \frac{\theta k^{\theta - 1}_T}{k^\theta_T}\\
k_T &= \frac{\theta \beta}{1 + \theta \beta}k^\theta_{T - 1}\\
k_{t + 1} &= \frac{\theta \beta (1 - (\theta \beta)^{T - t})}{1 - (\theta \beta)^{T - t + 1}} k^\theta_t\\
k_{t + 1} &= \theta \beta k_{t}^\theta
\end{align}
    \item $ $ 
    \begin{align}
    \overline{k} &= \theta \beta \overline{k}^\theta\\
\overline{k}^{1 - \theta} &= \theta \beta\\
\overline{k} &= (\theta \beta)^{\frac{1}{1 - \theta}}
\end{align}
    \item $ $
    \begin{align}
    u'(f(k) - k') &= \beta v'(k')\tag{FOC from Bellman}\\
U'(f(k_t) - k_{t + 1}) &= \beta U' (f(k_{t + 1}) - k_{t + 2})f'(k_{t + 1}) \tag{Euler Equation}\\
V'(S) &= R_k (k) + \beta V'(k') B_S(S) \tag{Envelope Condition \rd{Read up on this}}\\
\frac{1}{k^\theta - k'} &= \frac{\theta \beta}{1 - \theta \beta}\frac{1}{k'}\\
k' &= \theta \beta k^\theta
    \end{align}
  \end{enumerate}
  #+END_SRC 


  \newpage
* Problem 2

  \newpage
* Problem 3 (due to turn in)
