% Created 2020-10-13 Tue 14:53
% Intended LaTeX compiler: pdflatex
\documentclass[11pt]{article}
\usepackage[utf8]{inputenc}
\usepackage[T1]{fontenc}
\usepackage{graphicx}
\usepackage{grffile}
\usepackage{longtable}
\usepackage{wrapfig}
\usepackage{rotating}
\usepackage[normalem]{ulem}
\usepackage{amsmath}
\usepackage{textcomp}
\usepackage{amssymb}
\usepackage{capt-of}
\usepackage{hyperref}
\usepackage{amsthm}
\usepackage{url}
\newtheorem*{definition}{Definition}
\newtheorem*{example}{Example}
\newtheorem*{theorem}{Theorem}
\newtheorem*{exercise}{Exercise}
\newtheorem{question}{Question}
\usepackage[margin=1.25in]{geometry}
\usepackage{hyperref} % Required for adding links	and customizing them
\usepackage[dvipsnames]{xcolor}
\usepackage{booktabs}
\usepackage{enumitem}
\newcommand{\gr}{\textcolor{ForestGreen}}
\newcommand{\rd}{\textcolor{red}}
\newcommand{\R}{\mathbb{R}}
\newcommand{\frall}{\ \forall}
\author{Chris Ackerman}
\date{\today}
\title{Econ202A Assignment 1}
\hypersetup{
 pdfauthor={Chris Ackerman},
 pdftitle={Econ202A Assignment 1},
 pdfkeywords={},
 pdfsubject={},
 pdfcreator={Emacs 28.0.50 (Org mode 9.3)}, 
 pdflang={English}}
\begin{document}

\maketitle
\tableofcontents

\newpage
\section{Problem 1}
\label{sec:org9803f5a}
Consider the following problem solved be a representative agent:
  \begin{align*}
  \max \sum^\infty_{t = 0} &\beta^t \log c_t, \quad 0 < \beta < 1\\
\intertext{subject to}
c_t + k_{t + 1} &\le k^\theta_t, \quad 0 < \theta < 1,\\
k_0 &\text{ given.}
  \end{align*}
  \begin{enumerate}[label=(\alph*)]
    \item $ $
    \begin{align}
%     v(k_0) &= \max(u(c_0) + \beta v(k_1))\\
% v(k_0) &= \max(u(f(k_0) - k_1) + \beta v(k_1))\\
% u'(f(k_0) - k_1) &= \beta v'(k_1)\\
% F(k_t) &= k_t^\theta\\
U'(f(k_t) - k_{t + 1}) &= \beta U' (f(k_{t + 1}) - k_{t + 2})f'(k_{t + 1}) \tag{Euler Equation}\\
\frac{1}{k^\theta_t - k_{t + 1}} &= \beta \frac{\theta k^{\theta - 1}_{t + 1}}{k^\theta_{t + 1} - k_{t + 2}}\\
\frac{1}{k^\theta_{T - 1} - k_T} &= \beta \frac{\theta k^{\theta - 1}_T}{k^\theta_T}\\
k_T &= \frac{\theta \beta}{1 + \theta \beta}k^\theta_{T - 1}\\
k_{t + 1} &= \frac{\theta \beta (1 - (\theta \beta)^{T - t})}{1 - (\theta \beta)^{T - t + 1}} k^\theta_t\\
k_{t + 1} &= \theta \beta k_{t}^\theta
\end{align}
    \item $ $ 
    \begin{align}
    \overline{k} &= \theta \beta \overline{k}^\theta\\
\overline{k}^{1 - \theta} &= \theta \beta\\
\overline{k} &= (\theta \beta)^{\frac{1}{1 - \theta}}
\end{align}
    \item $ $
    \begin{align}
    u'(f(k) - k') &= \beta v'(k')\tag{FOC from Bellman}\\
U'(f(k_t) - k_{t + 1}) &= \beta U' (f(k_{t + 1}) - k_{t + 2})f'(k_{t + 1}) \tag{Euler Equation}\\
V'(S) &= R_k (k) + \beta V'(k') B_S(S) \tag{Envelope Condition \rd{Read up on this}}\\
\frac{1}{k^\theta - k'} &= \frac{\theta \beta}{1 - \theta \beta}\frac{1}{k'}\\
k' &= \theta \beta k^\theta
    \end{align}
  \end{enumerate}


\newpage
\section{Problem 2}
\label{sec:org6af34a8}

\newpage
\section{Problem 3 (due to turn in)}
\label{sec:orgc5d80d5}
\end{document}